theories/Infra/SafeFirst.v
@@ -1,47 +1,109 @@
-Require Import Util.
+Require Import CSet Util PidgeonHole OrderedTypeMax.
 
 Set Implicit Arguments.
 
-Section SafeFirst.
+Lemma asNat_ofNat_swap N `{NaturalRepresentation N} k m
+  : k = asNat m <-> ofNat k === m.
+Proof.
+  split; intros; subst.
+  - rewrite ofNat_asNat. reflexivity.
+  - rewrite <- H1. rewrite asNat_ofNat. reflexivity.
+Qed.
 
-  Hypothesis Q : nat -> Prop.
-  Inductive safe : nat -> Prop :=
-  | safe_here n : Q n -> safe n
-  | safe_after n : safe (S n) -> safe n.
+Lemma asNat_inj N `{NaturalRepresentationSucc N} m n
+  : asNat m = asNat n -> m === n.
+Proof.
+  intros.
+  remember (asNat m) as k.
+  general induction k.
+  - decide (m <<< n); eauto.
+    + exfalso. eapply order_respecting' in l.
+      instantiate (1:=H0) in l. omega.
+    + decide (n <<< m); eauto.
+      * exfalso. eapply order_respecting' in l.
+        instantiate (1:=H0) in l. omega.
+      * eapply lt_trans_eq; eauto.
+  - eapply asNat_ofNat_swap in Heqk.
+    eapply asNat_ofNat_swap in H2.
+    rewrite <- succ_ofNat in Heqk.
+    rewrite <- succ_ofNat in H2.
+    rewrite <- Heqk. rewrite <- H2.
+    reflexivity.
+Qed.
+
+Section SafeFirst.
+  Variable N : Type.
+  Context `{NaturalRepresentationSucc N}.
+
+  Hypothesis Q : N -> Prop.
+  Hypothesis Qpr : Proper (_eq ==> iff) Q.
+
+  Inductive safe : N -> Prop :=
+  | Isafe n : (~ (Q n) -> safe (succ n)) -> safe n.
+
+  Lemma safe_eq x y
+    : safe x -> x === y -> safe y.
+  Proof.
+    unfold Proper, respectful; intros.
+    general induction H2; eauto.
+    econstructor; intros. eapply H3; eauto.
+    rewrite H4. eauto. rewrite H4; eauto.
+  Qed.
+
+  Global Instance safe_proper
+    : Proper (_eq ==> iff) safe.
+  Proof.
+    unfold Proper, respectful; split; eauto using safe_eq.
+  Qed.
+
+  Lemma safe_antitone' (m n:nat)
+  : safe (ofNat n)
+    -> m < n
+    -> safe (ofNat m).
+  Proof.
+    intros.
+    general induction H3; eauto using safe.
+    - rewrite <- succ_ofNat in H2.
+      econstructor; eauto.
+    - rewrite <- succ_ofNat in H2.
+      assert (safe (ofNat m0)) by (econstructor; eauto).
+      eapply IHle in H4; eauto.
+  Qed.
 
   Lemma safe_antitone m n
-  : safe n
-    -> m < n
-    -> safe m.
+    : safe n
+      -> _lt m n
+      -> safe m.
   Proof.
-    intros. general induction H0; eauto using safe.
+    intros. rewrite <- ofNat_asNat.
+    rewrite <- ofNat_asNat in H2.
+    eapply order_respecting' in H3.
+    eapply safe_antitone'; eauto.
   Qed.
 
   Lemma exists_is_safe
   : (exists x, Q x) -> exists n, safe n.
   Proof.
-    intros. destruct H; eexists; eauto using safe.
+    intros. destruct H2; eexists; econstructor; intros.
+    exfalso; eauto.
   Qed.
 
-  Hypothesis comp  : forall n, Computable (Q n).
-
   Lemma safe_upward n
-  : safe n -> ~ Q n -> safe (S n).
+  : safe n -> ~ Q n -> safe (succ n).
   Proof.
-    intros; destruct H.
-    - destruct (H0 H).
-    - eapply H.
+    intros. inv H2. eauto.
   Defined.
 
-  Fixpoint safe_first n (s:safe n) : nat.
-  refine (if [ Q n ] then n else safe_first (S n) _).
-  destruct s; eauto. destruct (n0 H).
+  Hypothesis comp  : forall n, Computable (Q n).
+  Fixpoint safe_first n (s:safe n) : N.
+  refine (if [ Q n ] then n else safe_first (succ n) _).
+  destruct s; eauto.
   Defined.
 
-  Hypothesis P : nat -> Prop.
-  Hypothesis I : nat -> Prop.
+  Hypothesis P : N -> Prop.
+  Hypothesis I : N -> Prop.
   Hypothesis PQ : forall n, P n -> Q n.
-  Hypothesis Step : forall n, I n -> ~ Q n -> I (S n).
+  Hypothesis Step : forall n, I n -> ~ Q n -> I (succ n).
   Hypothesis Final : forall n , I n -> Q n -> P n.
 
   Fixpoint safe_first_spec n s
@@ -50,25 +112,26 @@ Section SafeFirst.
     unfold safe_first.
     destruct s.
     - simpl. destruct (decision_procedure (Q n)); eauto.
-    - cases; eauto.
   Qed.
 
 End SafeFirst.
 
-Fixpoint safe_first_ext P Q n
+Fixpoint safe_first_ext N `{NaturalRepresentationSucc N} P Q n
       (PC:forall n, Computable (P n))
       (QC:forall n, Computable (Q n))
       (PS:safe P n)
       (QS:safe Q n)
-      (EXT:(forall x, P x <-> Q x)) {struct PS}
+      (EXT:(forall x, P x <-> Q x)) {struct QS}
 : safe_first PC PS = safe_first QC QS.
 Proof.
-  destruct PS; destruct QS; simpl; repeat cases; eauto;
-  exfalso; firstorder.
+  destruct PS. destruct QS. simpl. repeat cases. reflexivity.
+  - exfalso. eapply n0. rewrite <- EXT. eauto.
+  - exfalso. eapply n0. rewrite EXT. eauto.
+  - eapply safe_first_ext. eauto.
 Qed.
 
-Lemma safe_impl (P Q: nat -> Prop) n
+Lemma safe_impl N `{NaturalRepresentationSucc N} (P Q: N -> Prop) n
 : safe P n -> (forall x, P x -> Q x) -> safe Q n.
 Proof.
-  intros. general induction H; eauto using safe.
+  intros. general induction H2; eauto 20 using @safe.
 Qed.
