theories/Infra/LeastFresh.v
@@ -1,0 +1,16 @@
+Require Import CSet Le Arith.Compare_dec.
+Require Import Plus Util Map Get Take LengthEq SafeFirst.
+Require Export PidgeonHole StableFresh OrderedTypeMax.
+
+Set Implicit Arguments.
+
+
+Class LeastFresh V `{NaturalRepresentation V} :=
+  {
+    least_fresh :> set V -> V;
+    least_fresh_spec : forall G, least_fresh G ∉ G;
+    least_fresh_least : forall G y, _lt y (least_fresh G) -> y ∈ G;
+    least_fresh_ext : forall G G', G [=] G' -> least_fresh G = least_fresh G'
+  }.
+
+Arguments LeastFresh V {H} {H0}.
