theories/Infra/OrderedTypeMax.v
@@ -1,0 +1,56 @@
+Require Import CSet.
+
+Definition nr_max X `{OrderedType X} (x y:X) :=
+  if [_lt x y] then y else x.
+
+Arguments nr_max {X} {H} x y.
+
+Instance nr_max_eq_proper X `{OrderedType X}
+  : Proper (_eq ==> _eq ==> _eq) nr_max.
+Proof.
+  unfold Proper, respectful; intros.
+  unfold nr_max. repeat cases; eauto.
+  exfalso. eapply NOTCOND. rewrite <- H1, <- H0. eauto.
+  exfalso. eapply NOTCOND. rewrite H1, H0. eauto.
+Qed.
+
+Lemma le_trans X `{OrderedType X} x y z
+  : ~ _lt x y -> ~ _lt y z -> ~ _lt x z.
+Proof.
+  intros. decide (x === y).
+  - rewrite e . eauto.
+  - eapply le_neq in n; eauto.
+    intro. eapply H1. etransitivity; eauto.
+Qed.
+
+Lemma lt_trans_eq X `{OrderedType X} x y
+  : ~ _lt x y -> ~ _lt y x -> _eq x y.
+Proof.
+  intros. decide (x === y); eauto.
+  - eapply le_neq in n; eauto.
+    exfalso. eauto.
+Qed.
+
+Lemma nr_max_sym X `{OrderedType X} (x y:X)
+  : nr_max x y === nr_max y x.
+Proof.
+  unfold nr_max; repeat cases; eauto.
+  - exfalso. assert (_lt x x) by (etransitivity; eauto).
+    eapply OrderedType.StrictOrder_Irreflexive in H0; eauto.
+  - eapply lt_trans_eq; eauto.
+Qed.
+
+Lemma nr_max_assoc X `{OrderedType X} (x y z:X)
+  : nr_max x (nr_max y z) === nr_max (nr_max x y) z.
+Proof.
+  unfold nr_max.
+  decide (_lt y z); decide (_lt x y).
+  - assert (_lt x z) by (etransitivity; eauto).
+    repeat cases; eauto.
+  - repeat cases; eauto.
+  - repeat cases; eauto.
+    exfalso; eauto.
+  - repeat cases; eauto.
+    exfalso; eauto.
+    eapply le_trans; eauto.
+Qed.
