theories/Infra/PidgeonHole.v
@@ -1,0 +1,298 @@
+Require Import CSet Le Arith.Compare_dec Plus Util.
+
+Class NaturalRepresentation X `{OrderedType X} :=
+  {
+    asNat : X -> nat;
+    ofNat : nat -> X;
+    ofNat_asNat : forall x, ofNat (asNat x) === x;
+    asNat_ofNat : forall n, asNat (ofNat n) === n;
+    order_respecting : forall x y, x < y <-> _lt (ofNat x) (ofNat y);
+    asNat_proper :> Proper (_eq ==> eq) asNat
+  }.
+
+Arguments asNat : simpl never.
+Arguments ofNat : simpl never.
+
+Arguments NaturalRepresentation X {H}.
+
+Ltac revert_except E :=
+  repeat match goal with
+         | [H : _ |- _] =>
+           match H with
+           | E => fail 1
+           | _ =>
+             match type of H with
+             | OrderedType _ => fail 1
+             | NaturalRepresentation _ => fail 1
+             | _ =>             revert H
+             end
+           end
+         end.
+
+Lemma order_respecting' X `{NaturalRepresentation X}
+  :  forall x y, asNat x < asNat y <-> _lt x y.
+Proof.
+  intros.
+  rewrite <- ofNat_asNat at 2.
+  rewrite <- (ofNat_asNat y) at 2.
+  eapply order_respecting.
+Qed.
+
+
+Class NaturalRepresentationSucc V `{NaturalRepresentation V} :=
+  {
+    succ : V -> V;
+    succ_asNat : forall x, asNat (succ x) = S (asNat x);
+    succ_ofNat : forall n:nat, succ (ofNat n) === ofNat (S n);
+    respect_lt :> Proper (_lt ==> _lt) succ;
+    respect_eq :> Proper (_eq ==> _eq) succ
+  }.
+
+Lemma all_in_lv_cardinal' X `{NaturalRepresentation X} (lv:set X) (n:nat)
+  : (forall m : X, _lt m (ofNat n) -> m \In lv) -> cardinal lv >= n.
+Proof.
+  general induction n; simpl.
+  - omega.
+  - exploit (IHn _ _ _ (lv \ singleton (ofNat n))).
+    + intros. cset_tac'.
+      * eapply H1. etransitivity; eauto.
+        eapply order_respecting. omega.
+      * rewrite <- H3 in H2. exfalso.
+        eapply OrderedType.StrictOrder_Irreflexive in H2. eauto.
+    + assert (EQ:lv [=] {ofNat n; lv \ singleton (ofNat n) }). {
+        exploit (H1 (ofNat n)); eauto.
+        eapply order_respecting. omega.
+        cset_tac.
+      }
+      rewrite EQ.
+      assert (ofNat n ∉ lv \ singleton (ofNat n)) by cset_tac.
+      erewrite cardinal_2; eauto. omega.
+      Grab Existential Variables.
+Qed.
+
+Arguments all_in_lv_cardinal' {X} {H} {H0} lv n.
+
+Lemma all_in_lv_cardinal X `{NaturalRepresentation X} (lv:set X) y
+  : (forall x : X, _lt x y -> x \In lv) -> cardinal lv >= asNat y.
+Proof.
+  intros. eapply all_in_lv_cardinal'.
+  intros m. rewrite ofNat_asNat. eauto.
+Qed.
+
+Arguments all_in_lv_cardinal {X} {H} {H0} lv y.
+
+Lemma neg_pidgeon_hole X `{NaturalRepresentation X} (lv:set X)
+  : (forall m : X, _lt m (ofNat (S (cardinal lv))) -> m \In lv) -> False.
+Proof.
+  intros. exploit (all_in_lv_cardinal' lv (S (cardinal lv))); eauto.
+  - omega.
+Qed.
+
+Instance NaturalRepresentationNat : NaturalRepresentation nat :=
+  {
+    asNat := fun x => x;
+    ofNat := fun x => x;
+  }.
+Proof.
+  - reflexivity.
+  - reflexivity.
+  - simpl. intros. omega.
+Defined.
+
+Definition posToNat (x:positive) :=
+  pred (Pos.iter_op Init.Nat.add x 1).
+
+Fixpoint natToPos (n : nat) : positive :=
+  match n with
+  | 0 => 1%positive
+  | 1 => 2%positive
+  | S (S _ as x) => Pos.succ (natToPos x)
+  end.
+
+Lemma succ_natToPos n
+  : Pos.succ (natToPos n) = natToPos (S n).
+Proof.
+  general induction n; simpl; eauto.
+Qed.
+
+Lemma natToPos_posToNat x
+  : natToPos (posToNat x) = x.
+Proof.
+  unfold posToNat. pattern x.
+  eapply Pos.peano_ind.
+  - simpl. reflexivity.
+  - intros. rewrite Pos.iter_op_succ.
+    + simpl. rewrite <- H at 2.
+      rewrite succ_natToPos.
+      erewrite <- S_pred. reflexivity.
+      eapply le_Pmult_nat.
+    + intros. omega.
+Qed.
+
+Lemma posToNat_natToPos n
+  : posToNat (natToPos n) = n.
+Proof.
+  unfold posToNat.
+  general induction n; eauto.
+  rewrite <- succ_natToPos.
+  rewrite Pos.iter_op_succ; [|intros;omega].
+  simpl. rewrite <- IHn at 2.
+  erewrite <- S_pred. reflexivity.
+  eapply le_Pmult_nat.
+Qed.
+
+Lemma lt_respect
+  : forall x y : nat, x < y <-> _lt (natToPos x) (natToPos y).
+Proof.
+  simpl. intros.
+  general induction x; simpl.
+  + split; intros.
+    * general induction y.
+      -- omega.
+      -- rewrite <- succ_natToPos.
+         eapply Pos.lt_1_succ.
+    * general induction y; simpl in *.
+      inv H. destruct y. omega. omega.
+  + split; intros.
+    * destruct x.
+      -- destruct y. omega.
+         exploit (IHx y); dcr. simpl in *.
+         destruct y. simpl in *. omega.
+         exploit H1; eauto. omega.
+         assert (2 = Pos.succ 1)%positive by reflexivity.
+         rewrite H3.
+         rewrite <- Pos.succ_lt_mono. eauto.
+      -- destruct y. omega. destruct y. omega.
+         edestruct (IHx (S y)). exploit H0. omega.
+         setoid_rewrite <- succ_natToPos at 2.
+         rewrite <- Pos.succ_lt_mono. eauto.
+    * destruct x.
+      -- destruct y; simpl in *. inv H.
+         destruct y. inv H. simpl in *. destruct y. hnf. reflexivity.
+         hnf. omega.
+      -- destruct y.
+         ++ setoid_rewrite <- succ_natToPos in H.
+           simpl in H. destruct (natToPos x); isabsurd.
+         ++ setoid_rewrite <- succ_natToPos in H at 2.
+           rewrite <- Pos.succ_lt_mono in H.
+           destruct y.
+           setoid_rewrite <- succ_natToPos in H.
+           simpl in H. destruct (natToPos x); isabsurd.
+           eapply IHx in H. omega.
+Qed.
+
+Instance NaturalRepresentationPositive : NaturalRepresentation positive :=
+  {
+    asNat := posToNat;
+    ofNat := natToPos;
+  }.
+Proof.
+  - eapply natToPos_posToNat.
+  - eapply posToNat_natToPos.
+  - eapply lt_respect.
+Defined.
+
+Class NaturalRepresentationMax V `{NaturalRepresentation V} :=
+  {
+    max : V -> V -> V;
+    max_asNat : forall x y, max x y === ofNat (Init.Nat.max (asNat x) (asNat y));
+    max_proper :> Proper (_eq ==> _eq ==> _eq) max
+  }.
+
+Arguments NaturalRepresentationMax V {H} {H0}.
+
+Smpl Create nr.
+
+Smpl Add
+     match goal with
+     | [ LT : context [ @_lt ?V _ _ _ ], NR:NaturalRepresentation ?V |- _ ] =>
+       setoid_rewrite <- (@order_respecting' V _ NR) in LT
+     | [ NR:NaturalRepresentation ?V |-  context [ @_lt ?V _ _ _ ] ] =>
+       setoid_rewrite <- (@order_respecting' V _ NR)
+     end : nr.
+
+Smpl Add
+     match goal with
+     | [ H: context [ @asNat ?V _ _ (@max ?V _ _ ?NRM _ _) ] |- _ ] =>
+       setoid_rewrite (@max_asNat V _ _ NRM) in H
+     | [ |- context [ @asNat ?V _ _ (@max ?V _ _ ?NRM _ _) ] ] =>
+       setoid_rewrite (@max_asNat V _ _ NRM)
+     end : nr.
+
+Smpl Add
+     match goal with
+     | [ LT : context [ @asNat ?V _ _ (@succ ?V _ _ ?NRS _) ] |- _ ] =>
+       setoid_rewrite (@succ_asNat V _ _ NRS) in LT
+     | [ |- context [ @asNat ?V _ _ (@succ ?V _ _ ?NRS _) ] ] =>
+       setoid_rewrite (@succ_asNat V _ _ NRS)
+     end : nr.
+
+Smpl Add
+     match goal with
+     | [ LT : context [ @asNat ?V _ ?NR (@ofNat ?V _ _ _) ] |- _ ] =>
+       setoid_rewrite (@asNat_ofNat V _ NR) in LT
+     | [ |- context [ @asNat ?V _ ?NR (@ofNat ?V _ _ _) ] ] =>
+       setoid_rewrite (@asNat_ofNat V _ NR)
+     end : nr.
+
+
+Ltac nr := repeat smpl nr.
+
+Instance NaturalRepresentationSuccNat : NaturalRepresentationSucc nat :=
+  {
+    succ := S
+  }.
+Proof.
+  - reflexivity.
+  - reflexivity.
+  - unfold Proper, respectful; cbn. intros; omega.
+Defined.
+
+Instance NaturalRepresentationMaxNat : NaturalRepresentationMax nat :=
+  {
+    max := Max.max
+  }.
+Proof.
+  - reflexivity.
+Defined.
+
+
+Instance NaturalRepresentationSuccPositive : NaturalRepresentationSucc positive :=
+  {
+    succ := Pos.succ
+  }.
+Proof.
+  - unfold asNat; simpl.
+    unfold posToNat; simpl.
+    intros. rewrite Pos.iter_op_succ; simpl.
+    erewrite <- S_pred. reflexivity.
+    eapply le_Pmult_nat. intros; omega.
+  - unfold ofNat. unfold NaturalRepresentationPositive.
+    intros. rewrite succ_natToPos. reflexivity.
+  - unfold Proper, respectful; cbn.
+    intros. rewrite <- Pos.succ_lt_mono. eauto.
+Defined.
+
+Lemma Posmax_asNat x y
+  : Pos.max x y === ofNat (Init.Nat.max (asNat x) (asNat y)).
+Proof.
+  pose proof (Pos.compare_spec x y).
+  unfold Pos.max. inv H.
+  - rewrite max_r; try omega. rewrite ofNat_asNat; eauto.
+  - rewrite max_r; try omega. rewrite ofNat_asNat; eauto.
+    edestruct (order_respecting' _ x y); eauto. simpl in *.
+    exploit H3. hnf. eauto. omega.
+  - rewrite Max.max_comm.
+    rewrite max_r; try omega. rewrite ofNat_asNat; eauto.
+    edestruct (order_respecting' _ y x); eauto. simpl in *.
+    exploit H3. eauto. omega.
+Defined.
+
+
+Instance NaturalRepresentationMaxPositive : NaturalRepresentationMax positive :=
+  {
+    max := Pos.max
+  }.
+Proof.
+  - intros. eapply Posmax_asNat.
+Defined.
